finish join chapter

src/beyond.v
@@ -1,6 +1,6 @@
 From Equations Require Import Equations.
 From Coq Require Import ssreflect ssrbool ssrfun.
-From mathcomp Require Import eqtype order ssrnat seq.
+From mathcomp Require Import eqtype order ssrnat seq path.
 From favssr Require Import prelude bintree bst redblack.
 
 Set Implicit Arguments.
@@ -29,117 +29,116 @@ Record ASetM2 (disp : unit) (T : orderType disp): Type :=
         _ : invar empty;
         _ : abs empty = [::];
 
-        _ : forall x s, invar s -> invar (insert x s);
-        _ : forall x s, invar s ->
-            perm_eq (abs (insert x s))
-                    (if x \in abs s then abs s else x :: abs s);
+        _ : forall x t, invar t -> invar (insert x t);
+        _ : forall x t, invar t ->
+            perm_eq (abs (insert x t))
+                    (if x \in abs t then abs t else x :: abs t);
 
-        _ : forall x s, invar s -> invar (delete x s);
-        _ : forall x s, invar s ->
-            perm_eq (abs (delete x s))
-                    (filter (predC1 x) (abs s));
+        _ : forall x t, invar t -> invar (delete x t);
+        _ : forall x t, invar t ->
+            perm_eq (abs (delete x t))
+                    (filter (predC1 x) (abs t));
 
-        _ : forall x s, invar s ->
-            isin s x = (x \in abs s);
+        _ : forall x t, invar t ->
+            isin t x = (x \in abs t);
 
-        _ : forall s1 s2, invar s1 -> invar s2 -> invar (uni s1 s2);
-        _ : forall s1 s2, invar s1 -> invar s2 ->
-            perm_eq (abs (uni s1 s2))
-                    (abs s1 ++ filter [predC mem (abs s1)] (abs s2));
+        _ : forall t1 t2, invar t1 -> invar t2 -> invar (uni t1 t2);
+        _ : forall t1 t2, invar t1 -> invar t2 ->
+            perm_eq (abs (uni t1 t2))
+                    (abs t1 ++ filter [predC mem (abs t1)] (abs t2));
 
-        _ : forall s1 s2, invar s1 -> invar s2 -> invar (int s1 s2);
-        _ : forall s1 s2, invar s1 -> invar s2 ->
-            perm_eq (abs (int s1 s2))
-                    (filter (mem (abs s2)) (abs s1));
+        _ : forall t1 t2, invar t1 -> invar t2 -> invar (int t1 t2);
+        _ : forall t1 t2, invar t1 -> invar t2 ->
+            perm_eq (abs (int t1 t2))
+                    (filter (mem (abs t2)) (abs t1));
 
-        _ : forall s1 s2, invar s1 -> invar s2 -> invar (dif s1 s2);
-        _ : forall s1 s2, invar s1 -> invar s2 ->
-            perm_eq (abs (dif s1 s2))
-                    (filter [predC mem (abs s2)] (abs s1))
+        _ : forall t1 t2, invar t1 -> invar t2 -> invar (dif t1 t2);
+        _ : forall t1 t2, invar t1 -> invar t2 ->
+            perm_eq (abs (dif t1 t2))
+                    (filter [predC mem (abs t2)] (abs t1))
         }.
 End ASetM2.
 
+(* TODO use a canonical structure? *)
+Record JoinSig (disp : unit) (X : orderType disp) (Y : Type) : Type :=
+  mkjoin {
+    join : tree (X*Y) -> X -> tree (X*Y) -> tree (X*Y);
+    inv : tree (X*Y) -> bool;
+    join_inorder : forall l a r,
+      inorder_a (join l a r) = inorder_a l ++ a :: inorder_a r;
+    bst_join : forall l a r,
+      all (< a) (inorder_a l) -> all (> a) (inorder_a r) ->
+      bst_a l -> bst_a r ->
+      bst_a (join l a r);
+    inv_leaf : inv leaf;
+    inv_join : forall l a r, inv l -> inv r -> inv (join l a r);
+    inv_node : forall l a b r, inv (Node l (a, b) r) -> inv l && inv r
+}.
+
 Section JustJoin.
-Context {disp : unit} {A : orderType disp} {B : Type}.
+Context {disp : unit} {X : orderType disp} {Y : Type} {j : JoinSig X Y}.
 
-Parameter join : tree (A*B) -> A -> tree (A*B) -> tree (A*B).
-Parameter inv : tree (A*B) -> bool.
-
-(* TODO perm_eq's should probably be strengthened to prop equality to simplify proofs *)
-(* see if the join implementations for RBT and 2-3 allow this *)
-
-Parameter join_inorder : forall l a r,
-  perm_eq (inorder_a (join l a r))
-          (inorder_a l ++ a :: inorder_a r).
-Parameter bst_join : forall l a r,
-  all (< a) (inorder_a l) -> all (> a) (inorder_a r) ->
-  bst_a l -> bst_a r ->
-  bst_a (join l a r).
-Parameter inv_leaf : inv empty_a.
-Parameter inv_join : forall l a r, inv l -> inv r -> inv (join l a r).
-Parameter inv_node : forall l a b r, inv (Node l (a, b) r) -> inv l && inv r.
-
-Fixpoint split (t : tree (A*B)) (x : A) : (tree (A*B) * bool * tree (A*B)) :=
+Fixpoint split (t : tree (X*Y)) (x : X) : (tree (X*Y) * bool * tree (X*Y)) :=
   if t is Node l (a,_) r then
       match cmp x a with
       | LT => let: (l1, b, l2) := split l x in
-              (l1, b, join l2 a r)
+              (l1, b, join j l2 a r)
       | EQ => (l, true, r)
       | GT => let: (r1, b, r2) := split r x in
-              (join l a r1, b, r2)
+              (join j l a r1, b, r2)
       end
-    else (empty_a, false, empty_a).
+    else (leaf, false, leaf).
 
-Fixpoint split_min (l : tree (A*B)) (a : A) (r : tree (A*B)) : (A * tree (A*B)) :=
+Fixpoint split_min (l : tree (X*Y)) (a : X) (r : tree (X*Y)) : (X * tree (X*Y)) :=
   if l is Node ll (al, _) rl then
       let: (m, l') := split_min ll al rl in
-      (m, join l' a r)
+      (m, join j l' a r)
     else (a, r).
 
-Definition join2 (l : tree (A*B)) (r : tree (A*B)) : tree (A*B) :=
+Definition join2 (l : tree (X*Y)) (r : tree (X*Y)) : tree (X*Y) :=
   if r is Node lr (ar, _) rr then
       let: (m, r') := split_min lr ar rr in
-      join l m r'
+      join j l m r'
   else l.
 
-Definition insert' (x : A) (t : tree (A*B)) : tree (A*B) :=
-  let: (l, b, r) := split t x in join l x r.
+Definition insert' (x : X) (t : tree (X*Y)) : tree (X*Y) :=
+  let: (l, b, r) := split t x in join j l x r.
 
-Definition delete' (x : A) (t : tree (A*B)) : tree (A*B) :=
+Definition delete' (x : X) (t : tree (X*Y)) : tree (X*Y) :=
   let: (l, b, r) := split t x in join2 l r.
 
-Fixpoint union (t1 t2 : tree (A*B)) : tree (A*B) :=
+Fixpoint union (t1 t2 : tree (X*Y)) : tree (X*Y) :=
   if t1 is Node l1 (a1,_) r1 then
     if t2 isn't Leaf then
       let: (l2, _, r2) := split t2 a1 in
-      join (union l1 l2) a1 (union r1 r2)
+      join j (union l1 l2) a1 (union r1 r2)
     else t1
   else t2.
 
-Fixpoint inter (t1 t2 : tree (A*B)) : tree (A*B) :=
+Fixpoint inter (t1 t2 : tree (X*Y)) : tree (X*Y) :=
   if t1 is Node l1 (a1,_) r1 then
     if t2 isn't Leaf then
       let: (l2, b2, r2) := split t2 a1 in
       let l' := inter l1 l2 in
       let r' := inter r1 r2 in
-      if b2 then join l' a1 r' else join2 l' r'
-    else empty_a
-  else empty_a.
+      if b2 then join j l' a1 r' else join2 l' r'
+    else leaf
+  else leaf.
 
-Fixpoint diff (t1 t2 : tree (A*B)) : tree (A*B) :=
+Fixpoint diff (t1 t2 : tree (X*Y)) : tree (X*Y) :=
   if t2 is Node l2 (a2,_) r2 then
     if t1 isn't Leaf then
       let: (l1, _, r1) := split t1 a2 in
       join2 (diff l1 l2) (diff r1 r2)
-    else empty_a
+    else leaf
   else t1.
 
 (* Correctness *)
 
 Lemma split_bst t x l b r :
   split t x = (l, b, r) -> bst_a t ->
-  [&& perm_eq (inorder_a l) (filter (< x) (inorder_a t)),
-      perm_eq (inorder_a r) (filter (> x) (inorder_a t)),
+  [&& inorder_a l == filter (< x) (inorder_a t),
+      inorder_a r == filter (> x) (inorder_a t),
       b == (x \in inorder_a t),
       bst_a l & bst_a r].
 Proof.
@@ -148,15 +147,14 @@ rewrite !filter_cat mem_cat inE /=; case Hxa: (cmp x a)=>/=.
 - move/cmp_lt: Hxa=>Hxa.
   case E: (split tl x)=>[[l1 bb] l2][El Eb Er]; rewrite {l1}El {bb}Eb in E.
   case/and4P=>Hal Har Hbl Hbr; rewrite Hxa ltNge le_eqVlt Hxa orbT /=.
-  case/and5P: (IHl _ _ E Hbl)=>Pl Pl2 /eqP -> -> Hbl2 /=.
+  case/and5P: (IHl _ _ E Hbl)=>/eqP Pl /eqP Pl2 /eqP -> -> Hbl2 /=.
   rewrite -Er; apply/and4P; split.
-  - apply: (perm_trans Pl).
-    rewrite -[X in perm_eq X _]cats0 perm_cat2l.
+  - rewrite Pl.
+    suff: [seq x0 <- inorder_a tr | x0 < x] = nil by move=>->; rewrite cats0.
     rewrite (eq_in_filter (a2:=pred0)); first by rewrite filter_pred0.
     move=>z /= /(allP Har) Hz; apply/negbTE; rewrite -leNgt.
     by apply/ltW/(lt_trans Hxa).
-  - apply: perm_trans; first by apply: join_inorder.
-    apply: perm_cat=>//; rewrite perm_cons.
+  - rewrite join_inorder Pl2.
     suff: all (> x) (inorder_a tr) by move/all_filterP=>{1}<-.
     by apply/sub_all/Har=>z Hz; apply/lt_trans/Hz.
   - suff: x \notin inorder_a tr.
@@ -165,29 +163,28 @@ rewrite !filter_cat mem_cat inE /=; case Hxa: (cmp x a)=>/=.
     apply/count_memPn/eqP; rewrite eqn0Ngt -has_count -all_predC.
     apply/sub_all/Har=>z /(lt_trans Hxa) /=.
     by rewrite lt_neqAle eq_sym; case/andP.
-   apply: bst_join=>//; rewrite (perm_all (<a) Pl2) all_filter.
+   apply: bst_join=>//; rewrite Pl2 all_filter.
    by apply/sub_all/Hal=>z /= Hz; apply/implyP.
 - move/cmp_eq: Hxa=>/eqP-> [-><-->] /and4P [Hal Har ->->] /=.
   rewrite eq_refl orbT /= andbT ltxx.
   move/all_filterP: (Hal)=>->; move/all_filterP: (Har)=>->.
   apply/andP; split.
-  - rewrite -[X in perm_eq X _]cats0 perm_cat2l.
+  - suff: [seq x <- inorder_a r | x < a] = nil by move=>->; rewrite cats0.
     rewrite (eq_in_filter (a2:=pred0)); first by rewrite filter_pred0.
     by move=>z /= /(allP Har) Hz; apply/negbTE; rewrite -leNgt; apply: ltW.
-  rewrite -[X in perm_eq X _]cat0s perm_cat2r.
+  suff: [seq x <- inorder_a l | a < x] = nil by move=>->.
   rewrite (eq_in_filter (a2:=pred0)); first by rewrite filter_pred0.
   by move=>z /= /(allP Hal) Hz; apply/negbTE; rewrite -leNgt; apply: ltW.
 move/cmp_gt: Hxa=>Hxa.
 case E: (split tr x)=>[[r1 bb] r2][El Eb Er]; rewrite {r2}Er {bb}Eb in E.
 case/and4P=>Hal Har Hbl Hbr; rewrite Hxa ltNge le_eqVlt Hxa orbT /=.
-case/and5P: (IHr _ _ E Hbr)=>Pr1 Pr /eqP -> Hbr1 -> /=.
+case/and5P: (IHr _ _ E Hbr)=>/eqP Pr1 /eqP Pr /eqP -> Hbr1 -> /=.
 rewrite andbT -El; apply/and4P; split.
-- apply: perm_trans; first by apply: join_inorder.
-  apply: perm_cat; last by rewrite perm_cons.
+- rewrite join_inorder Pr1.
   suff: all (< x) (inorder_a tl) by move/all_filterP=>{1}<-.
   by apply/sub_all/Hal=>z /= Hz; apply/lt_trans/Hxa.
-- apply: (perm_trans Pr).
-  rewrite -[X in perm_eq X _]cat0s perm_cat2r.
+- rewrite Pr.
+  suff: [seq x0 <- inorder_a tl | x < x0] = nil by move=>->.
   rewrite (eq_in_filter (a2:=pred0)); first by rewrite filter_pred0.
   move=>z /= /(allP Hal) Hz; apply/negbTE; rewrite -leNgt.
   by apply/ltW/(lt_trans Hz).
@@ -197,31 +194,30 @@ rewrite andbT -El; apply/and4P; split.
   apply/count_memPn/eqP; rewrite eqn0Ngt -has_count -all_predC.
   apply/sub_all/Hal=>z /= Hz; move: (lt_trans Hz Hxa).
   by rewrite lt_neqAle eq_sym; case/andP.
- apply: bst_join=>//; rewrite (perm_all (>a) Pr1) all_filter.
+ apply: bst_join=>//; rewrite Pr1 all_filter.
  by apply/sub_all/Har=>z /= Hz; apply/implyP.
 Qed.
 
 Lemma split_inv t x l b r :
-  split t x = (l, b, r) -> inv t ->
-  inv l && inv r.
+  split t x = (l, b, r) -> inv j t ->
+  inv j l && inv j r.
 Proof.
 elim: t l r=>/= [|tl IHl [a b'] tr IHr] l r; first by case=><-_<-; rewrite inv_leaf.
 case Hxa: (cmp x a)=>/=.
 - case E: (split tl x)=>[[l1 bb] l2][E1 Eb <-]; rewrite {l1}E1 {bb}Eb in E.
-  by case/inv_node/andP=>Hl Hr; case/andP: (IHl _ _ E Hl)=>->/= Hl2; apply: inv_join.
-- by case=>-> _ -> /inv_node.
+  by case/(inv_node (j:=j))/andP=>Hl Hr; case/andP: (IHl _ _ E Hl)=>->/= Hl2; apply: inv_join.
+- by case=>-> _ -> /(inv_node (j:=j)).
 case E: (split tr x)=>[[r1 bb] r2][<- Eb E2]; rewrite {r2}E2 {bb}Eb in E.
-by case/inv_node/andP=>Hl Hr; case/andP: (IHr _ _ E Hr)=>Hr1 ->/=; rewrite andbT; apply: inv_join.
+by case/(inv_node (j:=j))/andP=>Hl Hr; case/andP: (IHr _ _ E Hr)=>Hr1 ->/=; rewrite andbT; apply: inv_join.
 Qed.
 
 Lemma split_min_inorder l a r m t :
   split_min l a r = (m, t) ->
-  perm_eq (inorder_a l ++ a :: inorder_a r) (m :: inorder_a t).
+  inorder_a l ++ a :: inorder_a r = m :: inorder_a t.
 Proof.
 elim: l a r t=>/= [|ll IHl [al _] rl _] a r t; first by case=>->->.
 case Hsm: (split_min ll al rl)=>[m' l'][E' {t}<-]; rewrite {m'}E' in Hsm.
-move: (join_inorder l' a r); rewrite -(perm_cons m) perm_sym=>H.
-by apply/perm_trans/H; rewrite -cat_cons perm_cat2r; apply: IHl.
+by rewrite join_inorder (IHl _ _ _ Hsm).
 Qed.
 
 Lemma split_min_bst l a r m t :
@@ -231,33 +227,31 @@ Lemma split_min_bst l a r m t :
 Proof.
 elim: l a r t=>/= [|ll IHl [al _] rl _] a r t; first by case=>->->_->_->.
 case Hsm: (split_min ll al rl)=>[m' l'][E' {t}<-]; rewrite {m'}E' in Hsm.
-rewrite (perm_all (< a) (split_min_inorder Hsm))=>Haml' Har.
+rewrite (split_min_inorder Hsm) /= =>/andP [Hma Haml'] Har.
 case/and4P=>Halll Halrl Hbll Hbrl Hbr.
 case/andP: (IHl _ _ _ Hsm Halll Halrl Hbll Hbrl)=>Hbl' Hal'.
 apply/andP; split; first by apply: bst_join=>//; case/andP: Haml'.
-rewrite (perm_all (> m) (join_inorder l' a r)) all_cat Hal' /=.
-have Hma : m < a by case/andP: Haml'.
+rewrite join_inorder all_cat Hal' /=.
 by rewrite Hma /=; apply/sub_all/Har=>z /(lt_trans Hma).
 Qed.
 
 Lemma split_min_inv l a b r m t :
-  split_min l a r = (m, t) -> inv (Node l (a, b) r) ->
-  inv t.
+  split_min l a r = (m, t) -> inv j (Node l (a, b) r) ->
+  inv j t.
 Proof.
-move=>+ /inv_node /andP [].
+move=>+ /(inv_node (j:=j)) /andP [].
 elim: l a r t=>/= [|ll IHl [al bl] rl _] a r t; first by case=>_->.
 case Hsm: (split_min ll al rl)=>[m' l'][E' {t}<-]; rewrite {m'}E' in Hsm.
-case/inv_node/andP=>Hll Hrl Hr; apply: inv_join=>//.
+case/(inv_node (j:=j))/andP=>Hll Hrl Hr; apply: inv_join=>//.
 by apply: (IHl al rl).
 Qed.
 
 Lemma join2_inorder l r :
-  perm_eq (inorder_a (join2 l r)) (inorder_a l ++ inorder_a r).
+  inorder_a (join2 l r) = inorder_a l ++ inorder_a r.
 Proof.
 case: r=>/= [|lr [ar _] rr]; first by rewrite cats0.
 case Hsm: (split_min lr ar rr)=>[m r'].
-apply: (perm_trans (join_inorder l m r')); rewrite perm_cat2l perm_sym.
-by apply: split_min_inorder.
+by rewrite join_inorder (split_min_inorder Hsm).
 Qed.
 
 Lemma join2_bst l r :
@@ -266,12 +260,12 @@ Lemma join2_bst l r :
 Proof.
 move=>Hbl; case: r=>//=lr [ar _] rr /and4P [Halr Harr Hblr Hbrr].
 case Hsm: (split_min lr ar rr)=>[m r'].
-rewrite (perm_allrelr [eta <%O] _ (split_min_inorder Hsm)) allrel_consr; case/andP=>Ham Har'.
+rewrite (split_min_inorder Hsm) allrel_consr; case/andP=>Ham Har'.
 case/andP: (split_min_bst Hsm Halr Harr Hblr Hbrr)=>Hbr' Hmr'.
 by apply: bst_join.
 Qed.
 
-Lemma join2_inv l r : inv l -> inv r -> inv (join2 l r).
+Lemma join2_inv l r : inv j l -> inv j r -> inv j (join2 l r).
 Proof.
 move=>Hbl; case: r=>//=lr [ar br] rr H.
 case Hsm: (split_min lr ar rr)=>[m r']; apply: inv_join=>//.
@@ -279,7 +273,7 @@ by apply: (split_min_inv (b:=br) Hsm).
 Qed.
 
 (* TODO move to bst? not needed *)
-Lemma bst_a_uniq (t : tree (A*B)) : bst_a t -> uniq (inorder_a t).
+Lemma bst_a_uniq (t : tree (X*Y)) : bst_a t -> uniq (inorder_a t).
 Proof.
 elim: t=>//=l IHl [a b] r IHr /and4P [Hal Har /IHl Hl /IHr Hr].
 rewrite cat_uniq /= Hl Hr andbT /= negb_or -andbA; apply/and3P; split.
@@ -293,7 +287,7 @@ by apply/sub_all/Har=>z /=; rewrite eq_sym lt_neqAle; case/andP.
 Qed.
 
 (* TODO move to prelude *)
-Lemma eq_perm {T : eqType} (s1 s2 : seq A) : s1 = s2 -> perm_eq s1 s2.
+Lemma eq_perm {T : eqType} (s1 s2 : seq X) : s1 = s2 -> perm_eq s1 s2.
 Proof. by move=>->. Qed.
 
 (* union *)
@@ -310,23 +304,19 @@ elim: t1 t2=>/= [|l1 IHl [a1 b1] r1 IHr] t2.
 case/and4P=>Hal1 Har1 Hbl1 Hbr1.
 case E2: t2=>[|l2 [a2 b2] r2]; first by rewrite /= cats0.
 rewrite -{}E2=>H2; case Hs: (split t2 a1)=>[[l' b'] r'].
-case/and5P: (split_bst Hs H2)=>Hl' Hr' Hb' Hbl' Hbr'.
-apply: perm_trans; first by exact: join_inorder.
-move: (IHr _ Hbr1 Hbr'); rewrite -(perm_cons a1) => /(perm_cat (IHl _ Hbl1 Hbl'))=>H.
-apply: (perm_trans H); rewrite perm_catAC -cat_cons -!catA !perm_cat2l.
-move: (perm_cat (perm_filter [predC inorder_a r1] Hr') (perm_filter [predC inorder_a l1] Hl'))=>H'.
-apply/(perm_trans H')/perm_trans; last by apply/permEl/(perm_filterC (<= a1)).
-rewrite -!filter_predI perm_catC; apply: perm_cat.
-- apply/(@eq_perm A)/eq_filter=>z /=; rewrite mem_cat inE !negb_or.
-  case: (ltgtP z a1)=>//=; last by rewrite andbF.
-  rewrite andbT=>Hz; suff: z \notin inorder_a r1 by move=>->; rewrite andbT.
+case/and5P: (split_bst Hs H2)=>/eqP Hl' /eqP Hr' Hb' Hbl' Hbr'.
+rewrite join_inorder.
+move: (IHr _ Hbr1 Hbr'); rewrite -(perm_cons a1) =>/(perm_cat (IHl _ Hbl1 Hbl'))/perm_trans; apply.
+rewrite perm_catAC -cat_cons -!catA !perm_cat2l Hr' Hl'
+  perm_sym -(perm_filterC (<= a1)) -!filter_predI perm_catC; apply: perm_cat;
+apply/(@eq_perm X)/eq_filter=>z /=; rewrite mem_cat inE !negb_or;
+case: (ltgtP z a1)=>//=; try by [rewrite andbF]; rewrite andbT=>Hz.
+- suff: z \notin inorder_a l1 by move=>->.
   apply/count_memPn/eqP; rewrite eqn0Ngt -has_count -all_predC.
-  by apply/sub_all/Har1=>y /= /(lt_trans Hz); rewrite eq_sym lt_neqAle; case/andP.
-apply/(@eq_perm A)/eq_filter=>z /=; rewrite mem_cat inE !negb_or.
-case: (ltgtP a1 z)=>/=; try by rewrite andbF.
-rewrite andbT=>Hz; suff: z \notin inorder_a l1 by move=>->.
+  by apply/sub_all/Hal1=>y /= Hy; move: (lt_trans Hy Hz); rewrite lt_neqAle; case/andP.
+suff: z \notin inorder_a r1 by move=>->; rewrite andbT.
 apply/count_memPn/eqP; rewrite eqn0Ngt -has_count -all_predC.
-by apply/sub_all/Hal1=>y /= Hy; move: (lt_trans Hy Hz); rewrite lt_neqAle; case/andP.
+by apply/sub_all/Har1=>y /= /(lt_trans Hz); rewrite eq_sym lt_neqAle; case/andP.
 Qed.
 
 Lemma union_bst t1 t2 : bst_a t1 -> bst_a t2 -> bst_a (union t1 t2).
@@ -335,23 +325,23 @@ elim: t1 t2=>//=l1 IHl [a1 b1] r1 IHr t2.
 case/and4P=>Hal1 Har1 Hbl1 Hbr1.
 case E2: t2=>[|l2 [a2 b2] r2]; first by rewrite /= Hal1 Har1 Hbl1 Hbr1.
 rewrite -{}E2=>H2; case Hs: (split t2 a1)=>[[l' b'] r'].
-case/and5P: (split_bst Hs H2)=>Hl' Hr' Hb' Hbl' Hbr'.
+case/and5P: (split_bst Hs H2)=>/eqP Hl' /eqP Hr' Hb' Hbl' Hbr'.
 apply: bst_join.
 - rewrite (perm_all (< a1) (union_inorder Hbl1 Hbl')) all_cat all_filter Hal1 /=.
-  rewrite (perm_all _ Hl') all_filter /=.
+  rewrite Hl' all_filter /=.
   by apply/sub_all/all_predT=>z /= _; apply/implyP=>->; apply: implybT.
 - rewrite (perm_all (> a1) (union_inorder Hbr1 Hbr')) all_cat all_filter Har1 /=.
-  rewrite (perm_all _ Hr') all_filter /=.
+  rewrite Hr' all_filter /=.
   by apply/sub_all/all_predT=>z /= _; apply/implyP=>->; apply: implybT.
 - by apply: IHl.
 by apply: IHr.
 Qed.
 
-Lemma union_inv t1 t2 : inv t1 -> inv t2 -> inv (union t1 t2).
+Lemma union_inv t1 t2 : inv j t1 -> inv j t2 -> inv j (union t1 t2).
 Proof.
 elim: t1 t2=>//=l1 IHl [a1 b1] r1 IHr t2 H1.
 case E2: t2=>[|l2 [a2 b2] r2] //; rewrite -{}E2=>H2.
-case/inv_node/andP: H1=>Hl1 Hr1.
+case/(inv_node (j:=j))/andP: H1=>Hl1 Hr1.
 case Hs: (split t2 a1)=>[[l' b'] r'].
 case/andP: (split_inv Hs H2)=>Hl' Hr'.
 by apply: inv_join; [apply: IHl|apply: IHr].
@@ -360,8 +350,7 @@ Qed.
 (* intersection *)
 
 Lemma inter_inorder t1 t2 :
-  bst_a t1 ->
-  bst_a t2 ->
+  bst_a t1 -> bst_a t2 ->
   perm_eq (inorder_a (inter t1 t2))
           (filter (mem (inorder_a t2)) (inorder_a t1)).
 Proof.
@@ -372,22 +361,22 @@ case E2: t2=>[|l2 [a2 b2] r2].
   suff: filter (mem nil) s = [::] by move=>->.
   by rewrite -(filter_pred0 s); apply: eq_filter=>z /=; rewrite mem_filter.
 rewrite -{}E2=>H2; case Hs: (split t2 a1)=>[[l' b'] r'].
-case/and5P: (split_bst Hs H2)=>Hl' Hr' Hb' Hbl' Hbr'.
-case: {Hs}b' Hb'; rewrite eq_sym => /eqP Ha1.
-- apply: perm_trans; first by exact: join_inorder.
+case/and5P: (split_bst Hs H2)=>/eqP Hl' /eqP Hr' Hb' Hbl' Hbr'.
+case: {Hs}b' Hb'; rewrite eq_sym=>/eqP Ha1.
+- rewrite join_inorder.
   move: (IHr _ Hbr1 Hbr'); rewrite -(perm_cons a1) => /(perm_cat (IHl _ Hbl1 Hbl'))=>H.
   apply: (perm_trans H); rewrite filter_cat /= Ha1; apply: perm_cat.
-  - apply/(@eq_perm A)/eq_in_filter=>z /(allP Hal1) /= Hz.
-    by move/perm_mem: Hl' =>/(_ z) ->; rewrite mem_filter /= Hz.
-  rewrite perm_cons; apply/(@eq_perm A)/eq_in_filter=>z /(allP Har1) /= Hz.
-  by move/perm_mem: Hr' =>/(_ z) ->; rewrite mem_filter /= Hz.
-apply: perm_trans; first by exact: join2_inorder.
+  - apply/(@eq_perm X)/eq_in_filter=>z /(allP Hal1) /= Hz.
+    by rewrite Hl' mem_filter /= Hz.
+  rewrite perm_cons; apply/(@eq_perm X)/eq_in_filter=>z /(allP Har1) /= Hz.
+  by rewrite Hr' mem_filter /= Hz.
+rewrite join2_inorder.
 move: (IHr _ Hbr1 Hbr') => /(perm_cat (IHl _ Hbl1 Hbl'))=>H.
 apply: (perm_trans H); rewrite filter_cat /= Ha1; apply: perm_cat.
-- apply/(@eq_perm A)/eq_in_filter=>z /(allP Hal1) /= Hz.
-by move/perm_mem: Hl' =>/(_ z) ->; rewrite mem_filter /= Hz.
-apply/(@eq_perm A)/eq_in_filter=>z /(allP Har1) /= Hz.
-by move/perm_mem: Hr' =>/(_ z) ->; rewrite mem_filter /= Hz.
+- apply/(@eq_perm X)/eq_in_filter=>z /(allP Hal1) /= Hz.
+  by rewrite Hl' mem_filter /= Hz.
+apply/(@eq_perm X)/eq_in_filter=>z /(allP Har1) /= Hz.
+by rewrite Hr' mem_filter /= Hz.
 Qed.
 
 Lemma inter_bst t1 t2 : bst_a t1 -> bst_a t2 -> bst_a (inter t1 t2).
@@ -413,11 +402,11 @@ apply/allrel_filterl/allrel_filterr.
 by apply/sub_all/Hal1=>z /= Hz; apply/sub_all/Har1=>y Hy; apply/lt_trans/Hy.
 Qed.
 
-Lemma inter_inv t1 t2 : inv t1 -> inv t2 -> inv (inter t1 t2).
+Lemma inter_inv t1 t2 : inv j t1 -> inv j t2 -> inv j (inter t1 t2).
 Proof.
 elim: t1 t2=>//=l1 IHl [a1 b1] r1 IHr t2 H1.
 case E2: t2=>[|l2 [a2 b2] r2] //; rewrite -{}E2=>H2.
-case/inv_node/andP: H1=>Hl1 Hr1.
+case/(inv_node (j:=j))/andP: H1=>Hl1 Hr1.
 case Hs: (split t2 a1)=>[[l' b'] r'].
 case/andP: (split_inv Hs H2)=>Hl' Hr'.
 case: {Hs}b'.
@@ -428,32 +417,26 @@ Qed.
 (* difference *)
 
 Lemma diff_inorder t1 t2 :
-  bst_a t1 ->
-  bst_a t2 ->
+  bst_a t1 -> bst_a t2 ->
   perm_eq (inorder_a (diff t1 t2))
           (filter [predC mem (inorder_a t2)] (inorder_a t1)).
 Proof.
 elim: t2 t1=>/= [|l2 IHl [a2 _] r2 IHr] t1.
-- move=>H1 _; suff: filter [predC mem nil] (inorder_a t1) = inorder_a t1 by move=>->.
+- move=>_ _; suff: filter [predC mem nil] (inorder_a t1) = inorder_a t1 by move=>->.
   by apply/all_filterP/allP.
 case E1: t1=>[|l1 [a1 b1] r1] //; rewrite -{}E1=>H1.
 case/and4P=>Hal2 Har2 Hbl2 Hbr2.
 case Hs: (split t1 a2)=>[[l' b'] r'].
-case/and5P: (split_bst Hs H1)=>Hl' Hr' _ Hbl' Hbr'.
-apply: perm_trans; first by exact: join2_inorder.
-move: (IHr _ Hbr' Hbr2) => /(perm_cat (IHl _ Hbl' Hbl2))=>H.
-apply: (perm_trans H).
-move: (perm_cat (perm_filter [predC inorder_a l2] Hl') (perm_filter [predC inorder_a r2] Hr')) =>H'.
-apply/(perm_trans H')/perm_trans; last by apply/permEl/(perm_filterC (<= a2)).
-rewrite -!filter_predI; apply: perm_cat.
-- apply/(@eq_perm A)/eq_filter=>z /=; rewrite mem_cat inE !negb_or.
-  case: (ltgtP z a2)=>//=; last by rewrite andbF.
-  rewrite andbT=>Hz; suff: z \notin inorder_a r2 by move=>->; rewrite andbT.
+case/and5P: (split_bst Hs H1)=>/eqP Hl' /eqP Hr' _ Hbl' Hbr'.
+rewrite join2_inorder.
+move: (IHr _ Hbr' Hbr2) => /(perm_cat (IHl _ Hbl' Hbl2))/perm_trans; apply.
+rewrite Hl' Hr' perm_sym -(perm_filterC (<= a2)) -!filter_predI; apply: perm_cat;
+apply/(@eq_perm X)/eq_filter=>z /=; rewrite mem_cat inE !negb_or;
+case: (ltgtP a2 z)=>/=; try by [rewrite andbF]; rewrite andbT=>Hz.
+- suff: z \notin inorder_a r2 by move=>->; rewrite andbT.
   apply/count_memPn/eqP; rewrite eqn0Ngt -has_count -all_predC.
   by apply/sub_all/Har2=>y /= /(lt_trans Hz); rewrite eq_sym lt_neqAle; case/andP.
-apply/(@eq_perm A)/eq_filter=>z /=; rewrite mem_cat inE !negb_or.
-case: (ltgtP a2 z)=>/=; try by rewrite andbF.
-rewrite andbT=>Hz; suff: z \notin inorder_a l2 by move=>->.
+suff: z \notin inorder_a l2 by move=>->.
 apply/count_memPn/eqP; rewrite eqn0Ngt -has_count -all_predC.
 by apply/sub_all/Hal2=>y /= Hy; move: (lt_trans Hy Hz); rewrite lt_neqAle; case/andP.
 Qed.
@@ -461,29 +444,39 @@ Qed.
 Lemma diff_bst t1 t2 : bst_a t1 -> bst_a t2 -> bst_a (diff t1 t2).
 Proof.
 elim: t2 t1=>//=l2 IHl [a2 _] r2 IHr t1.
-case E1: t1=>[|l1 [a1 b1] r1] //; rewrite -{}E1=>H1.
+case E1: t1=>[|l1 [a1 b1] r1] //; rewrite -{l1 a1 b1 r1}E1=>H1.
 case/and4P=>Hal2 Har2 Hbl2 Hbr2.
 case Hs: (split t1 a2)=>[[l' b'] r'].
-case/and5P: (split_bst Hs H1)=>Hl' Hr' _ Hbl' Hbr'.
+case/and5P: (split_bst Hs H1)=>/eqP Hl' /eqP Hr' _ Hbl' Hbr'.
 apply: join2_bst.
 - by apply: IHl.
 - by apply: IHr.
 rewrite (perm_allrell _ _ (diff_inorder Hbl' Hbl2)) (perm_allrelr _ _ (diff_inorder Hbr' Hbr2)).
-apply/allrel_filterl/allrel_filterr; rewrite (perm_allrell _ _ Hl') (perm_allrelr _ _ Hr').
-rewrite /allrel all_filter.
+apply/allrel_filterl/allrel_filterr; rewrite Hl' Hr' /allrel all_filter.
 apply/sub_all/all_predT=>z /= _; apply/implyP=>Hz; rewrite all_filter.
 by apply/sub_all/all_predT=>y /= _; apply/implyP=>Hy; apply/lt_trans/Hy.
 Qed.
 
-Lemma diff_inv t1 t2 : inv t1 -> inv t2 -> inv (diff t1 t2).
+Lemma diff_inv t1 t2 : inv j t1 -> inv j t2 -> inv j (diff t1 t2).
 Proof.
 elim: t2 t1=>//=l2 IHl [a2 b2] r2 IHr t1.
 case E1: t1=>[|l1 [a1 b1] r1] //; rewrite -{}E1=>H1.
-case/inv_node/andP=>Hl2 Hr2.
+case/(inv_node (j:=j))/andP=>Hl2 Hr2.
 case Hs: (split t1 a2)=>[[l' b'] r'].
 case/andP: (split_inv Hs H1)=>Hl' Hr'.
 by apply: join2_inv; [apply: IHl|apply: IHr].
 Qed.
+
+(* Exercise 10.1 *)
+
+Fixpoint diff1 (t1 t2 : tree (X*Y)) : tree (X*Y) := leaf. (* FIXME *)
+
+Lemma diff1_inorder t1 t2 :
+  bst_a t1 -> bst_a t2 ->
+  perm_eq (inorder_a (diff1 t1 t2))
+          (filter [predC mem (inorder_a t2)] (inorder_a t1)).
+Proof.
+Admitted.
 
 End JustJoin.
 
@@ -502,11 +495,7 @@ joinL l x r with (ne_bhgt l r) := {
   | @Nd lr (xr, Black) rr _ _ => baliL (joinL l x lr) xr rr
   | Def => R l x r
   }.
-Proof.
-all: apply: ssrnat.ltP.
-- by rewrite addn1 ltnS; apply: leq_addr.
-by rewrite addn1 ltnS; apply: leq_addr.
-Qed.
+Proof. all: by apply: ssrnat.ltP; rewrite addn1 ltnS; apply: leq_addr. Qed.
 
 Equations? joinR (l : rbt T) (x : T) (r : rbt T) : rbt T by wf (size_tree l) lt :=
 joinR l x r with (ne_bhgt r l) := {
@@ -514,11 +503,7 @@ joinR l x r with (ne_bhgt r l) := {
   | @Nd ll (xl, Black) rl _ _ => baliR ll xl (joinR rl x r)
   | Def => R l x r
   }.
-Proof.
-all: apply: ssrnat.ltP.
-- by rewrite addn1 addnC ltnS; apply: leq_addr.
-by rewrite addn1 addnC ltnS; apply: leq_addr.
-Qed.
+Proof. all: by apply: ssrnat.ltP; rewrite addn1 addnC ltnS; apply: leq_addr. Qed.
 
 Definition joinRBT (l : rbt T) (x : T) (r : rbt T) : rbt T :=
   if (bh r < bh l)%N
@@ -584,11 +569,11 @@ by rewrite eqn_leq Hlr Hrl.
 Qed.
 
 Lemma joinL_inorder l a r :
-  perm_eq (inorder_a (joinL l a r)) (inorder_a l ++ a :: inorder_a r).
+  inorder_a (joinL l a r) = inorder_a l ++ a :: inorder_a r.
 Proof.
 funelim (joinL l a r); simp joinL; rewrite {}Heq //= e /=.
-- by rewrite -cat_cons catA perm_cat2r.
-by rewrite inorder_baliL -cat_cons catA perm_cat2r.
+- by rewrite H -catA.
+by rewrite inorder_baliL H -catA.
 Qed.
 
 Lemma bst_baliL (l : rbt T) a r :
@@ -633,12 +618,12 @@ Proof.
 funelim (joinL l a r); simp joinL; rewrite {}Heq /=; last by move=>->->->->.
 - rewrite {}e /= addn0 all_cat /= => Hal /and3P [Halr Hx _] Hbl /and4P [Halr' -> Hblr ->] E /=.
   rewrite andbT; apply/andP; split; last by apply: H.
-  rewrite (perm_all _ (joinL_inorder l x lr)) all_cat /= Hx Halr' /= andbT.
+  rewrite joinL_inorder all_cat /= Hx Halr' /= andbT.
   by apply/sub_all/Hal=>z /= Hz; apply/lt_trans/Hx.
 rewrite {}e /= in i *.
 rewrite all_cat /= => Hal /and3P [Halr Hx _] Hbl /and4P [Halr' Harr' Hblr Hbrr] _.
 apply: bst_baliL=>//; first by apply: H=>//; move: i; rewrite addn1 ltnS.
-rewrite (perm_all _ (joinL_inorder l x lr)) all_cat /= Hx Halr' /= andbT.
+rewrite joinL_inorder all_cat /= Hx Halr' /= andbT.
 by apply/sub_all/Hal=>z /= Hz; apply/lt_trans/Hx.
 Qed.
 
@@ -650,10 +635,10 @@ Lemma invc2_joinR l x r :
   invc2 (joinR l x r) && ((bh l != bh r) && (color l == Black) ==> invc (joinR l x r)).
 Proof.
 funelim (joinR l x r); simp joinR; rewrite {}Heq /=.
-- rewrite /invc2; rewrite {}e /= addn0 in i *.
+- rewrite /invc2; rewrite {}e /= in i *.
   have/negbTE->: (Red != Black) by [].
   rewrite andbF /= andbT => /and3P [/andP [_ Hrlb] -> Hcrl] Hcr /and3P [/eqP E1 Hhll Hhrl] Hhr E /=.
-  rewrite E1 in E i.
+  rewrite E1 addn0 in E i.
   case/andP: (H Hcrl Hcr Hhrl Hhr E)=>_; rewrite Hrlb !andbT /= => /implyP; apply.
   by move: i; rewrite ltn_neqAle E andbT eq_sym.
 - rewrite e /= in i *; rewrite eq_refl /= andbT.
@@ -685,7 +670,7 @@ Lemma invh_joinR l x r :
   invh (joinR l x r).
 Proof.
 funelim (joinR l x r); simp joinR; rewrite {}Heq /=.
-- rewrite {Heqcall l i}e /= addn0; case/and3P=>/eqP E1 -> Hrl Hr E /=; rewrite E1 in E *.
+- rewrite {Heqcall l i}e /=; case/and3P=>/eqP E1 -> Hrl Hr E /=; rewrite E1 addn0 in E *.
   by rewrite eq_sym; apply/andP; split; [apply: bh_joinR | apply: H].
 - rewrite {Heqcall l}e /= in i *; case/and3P=>/eqP E1 Hll Hrl ? ?.
   move: i; rewrite addn1 ltnS E1=>E.
@@ -696,11 +681,11 @@ by rewrite eqn_leq Hlr Hrl.
 Qed.
 
 Lemma joinR_inorder l a r :
-  perm_eq (inorder_a (joinR l a r)) (inorder_a l ++ a :: inorder_a r).
+  inorder_a (joinR l a r) = inorder_a l ++ a :: inorder_a r.
 Proof.
 funelim (joinR l a r); simp joinR; rewrite {}Heq //= e /=.
-- by rewrite -catA perm_cat2l perm_cons.
-by rewrite inorder_baliR -catA perm_cat2l perm_cons.
+- by rewrite H -catA.
+by rewrite inorder_baliR H -catA.
 Qed.
 
 Lemma bst_baliR (l : rbt T) a r :
@@ -741,20 +726,19 @@ Proof.
 funelim (joinR l a r); simp joinR; rewrite {}Heq /=; last by move=>->->->->.
 - rewrite {}e /= all_cat /= => /and3P [_ Hx Harl] Har /and4P [-> Harl' -> Hbrl] Hbr /=.
   apply/andP; split; last by apply: H.
-  rewrite (perm_all _ (joinR_inorder rl x r)) all_cat /= Hx Harl' /=.
+  rewrite joinR_inorder all_cat /= Hx Harl' /=.
   by apply/sub_all/Har=>z /= /(lt_trans Hx).
 rewrite {}e /= in i *.
 rewrite all_cat /= => /and3P [_ Hx Harl] Har /and4P [Hall' Harl' Hbll Hbrl] Hbr.
 apply: bst_baliR=>//; first by apply: H.
-rewrite (perm_all _ (joinR_inorder rl x r)) all_cat /= Hx Harl' /=.
+rewrite joinR_inorder all_cat /= Hx Harl' /=.
 by apply/sub_all/Har=>z /= /(lt_trans Hx).
 Qed.
 
-(* joinRBT *)
+(* join *)
 
-Lemma joinRBT_inorder l a r :
-  perm_eq (inorder_a (joinRBT l a r))
-          (inorder_a l ++ a :: inorder_a r).
+Lemma join_inorderRBT l a r :
+  inorder_a (joinRBT l a r) = inorder_a l ++ a :: inorder_a r.
 Proof.
 rewrite /joinRBT; case: ifP=>_.
 - by rewrite inorder_paint; exact: joinR_inorder.
@@ -769,22 +753,19 @@ Lemma bst_joinRBT l a r :
   bst_a l -> bst_a r ->
   bst_a (joinRBT l a r).
 Proof.
-move=>Hal Har Hbl Hbr; rewrite /joinRBT; case: ifP=>E.
+move=>Hal Har Hbl Hbr; rewrite /joinRBT; case: ltnP=>E.
 - by rewrite bst_paint; apply: bst_joinR.
 case: ifP=>_ /=; last by rewrite Hal Har Hbl Hbr.
-rewrite bst_paint; apply: bst_joinL=>//.
-by move/negbT: E; rewrite -leqNgt.
+by rewrite bst_paint; apply: bst_joinL.
 Qed.
 
-Definition invr (t : rbt T) := invc t && invh t.
-
-Lemma invr_leaf : invr empty_a.
+Lemma invch_leaf : invch (@Leaf (T*col)).
 Proof. by []. Qed.
 
-Lemma invr_joinRBT l a r : invr l -> invr r -> invr (joinRBT l a r).
+Lemma invch_joinRBT l a r : invch l -> invch r -> invch (joinRBT l a r).
 Proof.
-rewrite /invr; case/andP=>Hcl Hhl; case/andP=>Hcr Hhr.
-rewrite /joinRBT; case: ltnP=>[/ltnW|] E.
+case/andP=>Hcl Hhl; case/andP=>Hcr Hhr.
+rewrite /joinRBT /invch; case: ltnP=>[/ltnW|] E.
 - apply/andP; split; last by apply/invh_paint/invh_joinR.
   by case/andP: (invc2_joinR a Hcl Hcr Hhl Hhr E); rewrite /invc2.
 case: ltnP=>E' /=; last by rewrite Hcl Hcr Hhl Hhr /= andbT eqn_leq E E'.
@@ -792,7 +773,162 @@ apply/andP; split; last by apply/invh_paint/invh_joinL.
 by case/andP: (invc2_joinL a Hcl Hcr E); rewrite /invc2.
 Qed.
 
-Lemma invr_node l a b r : invr (Node l (a, b) r) -> invr l && invr r.
-Proof. by rewrite /invr /= -!andbA; case/and6P=>_->->_->->. Qed.
+Lemma invch_node (l : rbt T) a b r : invch (Node l (a, b) r) -> invch l && invch r.
+Proof. by rewrite /invch /= -!andbA; case/and6P=>_->->_->->. Qed.
+
+Definition JoinRBT :=
+  @mkjoin _ _ _
+    joinRBT
+    invch
+    join_inorderRBT
+    bst_joinRBT
+    invch_leaf
+    invch_joinRBT
+    invch_node.
 
 End JoiningRedBlackTrees.
+
+Section RBTSetJoin.
+Context {disp : unit} {T : orderType disp}.
+
+Definition invariant' (t : rbt T) := bst_list_a t && invch t.
+
+Lemma invariant_empty' : invariant' leaf.
+Proof. by []. Qed.
+
+Corollary invariant_insert' x (t : rbt T) :
+  invariant' t -> invariant' (insert x t).
+Proof.
+rewrite /invariant' /bst_list_a => /andP [H1 H2].
+apply/andP; split; last by apply: inv_insert.
+by rewrite inorder_insert //; apply: ins_list_sorted.
+Qed.
+
+Corollary inorder_insert_list' x (t : rbt T) :
+  invariant' t ->
+  perm_eq (inorder_a (insert x t))
+          (if x \in inorder_a t then inorder_a t else x :: inorder_a t).
+Proof.
+rewrite /invariant' /bst_list_a => /andP [H1 _].
+by rewrite inorder_insert //; apply: inorder_ins_list.
+Qed.
+
+Corollary invariant_delete' x (t : rbt T) :
+  invariant' t -> invariant' (delete x t).
+Proof.
+rewrite /invariant' /bst_list_a => /andP [H1 H2].
+apply/andP; split; last by apply: inv_delete.
+by rewrite inorder_delete //; apply: del_list_sorted.
+Qed.
+
+Corollary inorder_delete_list' x (t : rbt T) :
+  invariant' t ->
+  perm_eq (inorder_a (delete x t))
+          (filter (predC1 x) (inorder_a t)).
+Proof.
+rewrite /invariant' /bst_list_a => /andP [H1 H2].
+by rewrite inorder_delete //; apply: inorder_del_list.
+Qed.
+
+Lemma inv_isin_list' x (t : rbt T) :
+  invariant' t ->
+  isin_a t x = (x \in inorder_a t).
+Proof. by rewrite /invariant' => /andP [H1 _]; apply: inorder_isin_list_a. Qed.
+
+Corollary invariant_union' (t1 t2 : rbt T) :
+  invariant' t1 -> invariant' t2 -> invariant' (union (j:=JoinRBT) t1 t2).
+Proof.
+rewrite /invariant' /bst_list_a => /andP [H11 H12] /andP [H21 H22].
+apply/andP; split; last by apply: (union_inv (j:=JoinRBT)).
+by apply/bst_to_list_a/union_bst; apply/bst_to_list_a.
+Qed.
+
+Corollary inorder_union' (t1 t2 : rbt T) :
+  invariant' t1 -> invariant' t2 ->
+  perm_eq (inorder_a ((union (j:=JoinRBT)) t1 t2))
+          (inorder_a t1 ++ filter [predC mem (inorder_a t1)] (inorder_a t2)).
+Proof.
+rewrite /invariant' /bst_list_a => /andP [H11 _] /andP [H21 _].
+by apply: union_inorder; apply/bst_to_list_a.
+Qed.
+
+Corollary invariant_inter' (t1 t2 : rbt T) :
+  invariant' t1 -> invariant' t2 -> invariant' (inter (j:=JoinRBT) t1 t2).
+Proof.
+rewrite /invariant' /bst_list_a => /andP [H11 H12] /andP [H21 H22].
+apply/andP; split; last by apply: (inter_inv (j:=JoinRBT)).
+by apply/bst_to_list_a/inter_bst; apply/bst_to_list_a.
+Qed.
+
+Corollary inorder_inter' (t1 t2 : rbt T) :
+  invariant' t1 -> invariant' t2 ->
+  perm_eq (inorder_a ((inter (j:=JoinRBT)) t1 t2))
+          (filter (mem (inorder_a t2)) (inorder_a t1)).
+Proof.
+rewrite /invariant' /bst_list_a => /andP [H11 _] /andP [H21 _].
+by apply: inter_inorder; apply/bst_to_list_a.
+Qed.
+
+Corollary invariant_diff' (t1 t2 : rbt T) :
+  invariant' t1 -> invariant' t2 -> invariant' (diff (j:=JoinRBT) t1 t2).
+Proof.
+rewrite /invariant' /bst_list_a => /andP [H11 H12] /andP [H21 H22].
+apply/andP; split; last by apply: (diff_inv (j:=JoinRBT)).
+by apply/bst_to_list_a/diff_bst; apply/bst_to_list_a.
+Qed.
+
+Corollary inorder_diff' (t1 t2 : rbt T) :
+  invariant' t1 -> invariant' t2 ->
+  perm_eq (inorder_a ((diff (j:=JoinRBT)) t1 t2))
+          (filter [predC mem (inorder_a t2)] (inorder_a t1)).
+Proof.
+rewrite /invariant' /bst_list_a => /andP [H11 _] /andP [H21 _].
+by apply: diff_inorder; apply/bst_to_list_a.
+Qed.
+
+Definition SetRBT2 :=
+  @ASetM2.make _ _ (rbt T)
+    leaf insert delete isin_a
+    (union (j:=JoinRBT)) (inter (j:=JoinRBT)) (diff (j:=JoinRBT))
+    inorder_a invariant'
+    invariant_empty' erefl
+    invariant_insert' inorder_insert_list'
+    invariant_delete' inorder_delete_list'
+    inv_isin_list'
+    invariant_union' inorder_union'
+    invariant_inter' inorder_inter'
+    invariant_diff' inorder_diff'.
+
+End RBTSetJoin.
+
+(* Exercise 10.2 *)
+
+From favssr Require Import twothree.
+
+Section Joining23Trees.
+Context {disp : unit} {T : orderType disp}.
+
+Equations? join23L (l : tree23 T) (x : T) (r : tree23 T) : upI T by wf (size23 r) lt :=
+join23L l x r => TI l. (* FIXME *)
+Proof.
+Qed.
+
+Equations? join23R (l : tree23 T) (x : T) (r : tree23 T) : upI T by wf (size23 l) lt :=
+join23R l x r => TI r. (* FIXME *)
+Proof.
+Qed.
+
+Definition join23 (l : tree23 T) (x : T) (r : tree23 T) : tree23 T :=
+  l. (* FIXME *)
+
+Lemma complete_join23 l x r :
+  complete23 l -> complete23 r -> complete23 (join23 l x r).
+Proof.
+Admitted.
+
+Lemma join_inorder23 l a r :
+  inorder23 (join23 l a r) = inorder23 l ++ a :: inorder23 r.
+Proof.
+Admitted.
+
+End Joining23Trees.
